\documentclass[12pt, A4]{report}

\usepackage{amsmath}
\usepackage{amssymb}
\usepackage{bm}
\usepackage{fancyhdr}
\usepackage[margin=0.75in]{geometry}
\usepackage[utf8]{inputenc}
\usepackage{tikz}
\usetikzlibrary{calc}

% Configuration
\title{AP Calculus Practice Problems}
\author{Arnav Patri}

\pagestyle{fancy}
\fancyhead{}
	\fancyhead[L]{\leftmark}
	\fancyhead[R]{Arnav Patri}
	\renewcommand{\chaptermark}[1]{\markboth{#1}{}}

% Symbols
\renewcommand{\d}{\text{d}}

\begin{document}
	\chapter*{Volume: Disk/Washer\markboth{Volume: Disk/Washer}{}}
		\section*{Sources}
			\subsection*{Calculus: Early Transcendentals 9$^{\textbf{th}}$ Edition}
				\begin{enumerate}
					\item
						6.2 Exercise 12
					\item
						6.2 Exercise 15
					\item 
						6.2 Exercise 1
					\item
						6.2 Exercise 17
					\item
						6.2 Exercise 24
				\end{enumerate}
			\subsection*{AP Calculus Exams}
				\begin{enumerate}
					\setcounter{enumi}{5}
					\item
						2021 AB FRQ 3(c)
				\end{enumerate}
			\newpage
		\section*{Problems}
			If no instructions are given, evaluate the volume of the solid generated by revolving the region bounded by the given equations about the specified line using the disk/washer method.
			\begin{enumerate}
				\item
					\[
						\left.\begin{aligned}
							y &= 0 &
								y &= \frac{1}{x} \\
							x &= 1 &
								x &= 4
						\end{aligned}\,\right|\, y = 0
					\]
				\item
					\[
						\left.\begin{aligned}
							y &= \frac{x^2}{4} &
								y &= 9 \\
							x &= 0
						\end{aligned}\,\right|\, x = 0
					\]
				\item
					\[
						\left.\begin{aligned}
							y &= 0 & 
								y &= x^2 + 5 \\
							x &= 0 &
								x &= 3
						\end{aligned}\,\right|\, y = 0
					\]
				\item
					\[
						\left.\begin{aligned}
							y &= x^2 \\
							y &= 2x 
						\end{aligned}\,\right|\, x = 0
					\]
				\item
					\[
						\left.\begin{aligned}
							y &= \sin x &
								y &= \cos x \\
							x &\ge 0 & 
								x &\le \frac{\pi}{4}
						\end{aligned}\,\right|\, y = -1
					\]
				\item
					\[f(x) = cx\sqrt{4 - x^2}\]
					The solid of revolution generated by rotating the area bounded by $f$ and the $x$-axis in the first quadrant about the $x$-axis is equal to $2\pi$. Solve for $c$, given that it is a positive constant.
				\item
					%TODO Hyperbola bounded by asymptotes
				\item
					\[
						\left.\begin{aligned}
							x^2 + y^2 &= r^2 & 
								\frac{x^2}{a^2} + \frac{y^2}{b^2} &= 1 
								\mid a, b > r > 0\\
							\text{(a) } y &= 0
						\end{aligned}\,\right|\,
						\begin{aligned}
							\text{(a) } &y = 0 \\
							\text{(b) } &y = b
						\end{aligned}
					\]
			\end{enumerate}
			\newpage
		\section*{Solutions}
			\begin{enumerate}
				\item
					\begin{align*}
						V &= \pi\int_1^4\left(\frac{1}{x}\right)^2\d x
								 = \pi\left[-\frac{1}{x}\right]_1^4
								 = \pi\left[-\frac{1}{4} -\left(-\frac{1}{1}\right)\right]
								 = \frac{3\pi}{4} \\
					\end{align*}
				\item
					\begin{align*}
						y &= \frac{x^2}{4} \implies x = 2\sqrt{y} \\
						y_1 &= 2\sqrt{0} = 0 \\
						V &= \pi\int_0^9\left(2\sqrt{y}\right)^2\d y = \pi\left[2y^2\right]_0^9 = 2(81)\pi = 162\pi
					\end{align*}
				\item
					\begin{align*}
						V &= \pi\int_0^3\left(x^2 + 5\right)^2\d x 
								= \pi\int_{0}^3\left[x^4 + 10x^2 + 25\right]\d x 
								= \pi\left[\frac{x^5}{5} + \frac{10x^3}{3} + 25x\right]_0^3 \\
							&= \pi\left[\frac{3^5}{5} + \frac{10(3)^3}{3} + 25(3) - (0)\right] 
								= \pi\left[\frac{243}{5} + 90 + 75\right] 
								= \frac{\pi(243 + 825)}{5} 
								= \frac{1068\pi}{5} \\
					\end{align*}
				\item
					\begin{align*}
						y &= x^2 \implies x = \sqrt{y} \qquad 
								y = 2x \implies x = \frac{y}{2} \\
						\sqrt{y} &= \frac{y}{2} 
								\implies 4y = y^2 
								\implies 0 = y(y - 4) 
								\implies y_1 = 0, y_2 = 4 \\
						V &= \pi\int_0^4\left[\left(\sqrt{y}\right)^2 - \left(\frac{y}{2}\right)^2\right]\d y
							 	= \pi\int_0^4\left[y - \frac{y^2}{4}\right]\d y
							 	= \pi\left[\frac{y^2}{2} - \frac{y^3}{12}\right]_0^4 \\
							 &= \pi\left[\frac{y^2(6 - y)}{12}\right]_0^4
							 	= \pi\left[\frac{4^2(6 - 4)}{12} - (0)\right]
							 	= \pi\left[\frac{16(2)}{12}\right]
							 	= \frac{8\pi}{3}
					\end{align*}
				\item
					\begin{align*}
						\sin x &= \cos x 
								\implies x = \frac{\pi}{4} \\
						V &= \pi\int_0^{\pi/4}\left[(\cos x + 1)^2 - (\sin x + 1)^2\right]\d x \\
							&= \pi\int_0^{\pi/4}\left[\cos^2x + 2\cos x + 1 - \sin^2 x - 2\sin x - 1\right]\d x \\
							&= \pi\int_0^{\pi/4}\left[\cos(2x) + 2\cos x - 2\sin x\right]\d x
								= \pi\left[\frac{\sin(2x)}{2} + 2\sin x + 2\cos x\right]_0^{\pi/4} \\
							&= \pi\left[\frac{1}{2} + \sqrt{2} + \sqrt{2} - (0 + 0 + 2)\right]
								= \frac{(4\sqrt{2} - 3)\pi}{2}
					\end{align*}
				\item
					\begin{align*}
						0 &= cx\sqrt{4 - x^2} \implies 
							\begin{cases}
	 							x = 0 \\
	 							\sqrt{4 - x^2} = 0 &\implies 4 - x^2 = 0 
	 								\implies 4 = x^2 
	 								\implies x = 2
							\end{cases} \\
						2\pi &= \pi\int_0^2\left(cx\sqrt{4 - x^2}\right)^2\d x
									= \pi\int_0^2\left[c^2x^2(4 - x^2)\right]\d x
									= \pi\int_0^4\left[4c^2x^2 - c^2x^4\right]\d x \\
								&= \pi\left[\frac{4c^2x^3}{3} - \frac{c^2x^5}{5}\right]_0^2
									= \pi\left[\frac{4c^2(2)^3}{3} - \frac{c^2(2)^5}{5} - (0)\right]
									= \pi\left[\frac{32c^2}{3} - \frac{32c^2}{5}\right] \\
							2 &= 32c^2\left(\frac{1}{3} - \frac{1}{5}\right) 
									= \frac{64c^2}{15} \\
							c &= \sqrt{\frac{30}{64}} = \sqrt{\frac{15}{32}}
					\end{align*}
				\newpage\item
					\[\begin{tikzpicture}
						\draw[thick, <->] (-3.5, 0) -- (3.5, 0) node[anchor = west]{$x$};
						\draw[thick, <->] (0, -2.5) -- (0, 2.5) node[anchor = south]{$y$};
							\node[anchor = north east]{$O$};
						\draw[] circle[radius = 1];
							\node[anchor = south west] at (1, 0) {$r$};
						\draw[] ellipse(3cm and 2cm);
							\node[anchor = south west] at (0, 2) {$b$};
							\node[anchor = south west] at (3, 0) {$a$};
						\draw[dashed, <->] (-3.5, 2) -- (3.5, 2);
						\node[anchor = north] at (0, -2.5) {This graph assumes $a > b$, which need not be the case.};
					\end{tikzpicture}\]
					\[
						x^2 + y^2 = r^2 
								\implies y = \sqrt{r^2 - x^2} \qquad 
								\frac{x^2}{a^2} + \frac{y^2}{b^2} = 1 
									\implies y = b\sqrt{1 - \frac{x^2}{a^2}} = \frac{b\sqrt{a^2 - x^2}}{a}
					\]
					\begin{enumerate}
						\item
							\begin{align*}
								V_1 &= \pi\int_0^r\left[\left(\frac{b\sqrt{a^2 - x^2}}{a}\right)^2 - \left(\sqrt{r^2 - x^2}\right)^2\right]\d x
										= \pi\int_0^r\left[\frac{b^2(a^2 - x^2)}{a^2} - (r^2 - x^2)\right]\d x \\
									&= \pi\int_0^r\left[\frac{a^2(b^2 - r^2) + x^2(a^2 - b^2)}{a^2}\right]\d x 
										= \pi\left[\frac{a^2x(b^2 - r^2)}{a^2} + \frac{x^3(a^2 - b^2)}{3a^2}\right]_0^4 \\
									&= \pi\left[\frac{3a^2x(b^2 - r^2) + x^3(a^2 - b^2)}{3a^2}\right]_0^r
										= \pi\left[\frac{3a^2r(b^2 - r^2) + r^3(a^2 - b^2)}{3a^2}\right] \\
									&= \pi\left[\frac{3a^2b^2r - 3a^2r^3 + a^2r^3 - b^2r^3}{3a^2}\right]
										= \pi\left(\frac{3a^2b^2r - 2a^2r^3 - b^2r^3}{3a^2}\right) \\
								V_2 &= \pi\int_r^a\left(\frac{b\sqrt{a^2 - x^2}}{a}\right)^2\d x
										= \pi\int_r^a\left[\frac{b^2(a^2 - x^2)}{a^2}\right]\d x  = \pi\int_r^a\left[\frac{a^2b^2 - b^2x^2}{a^2}\right]\d x \\
									&= \pi\left[\frac{a^2b^2x}{a^2} - \frac{b^2x^3}{3a^2}\right]_r^a 
										= \pi\left[\frac{3a^2b^2x - b^2x^3}{3a^2}\right]_r^a 
										= \left[\frac{3a^3b^2 - b^2a^3}{3a^2} - \left(\frac{3a^2b^2r -b^2r^3}{3a^2}\right)\right] \\
									&= \pi\left(\frac{2a^3b^2 -3a^2b^2r + b^2r^3}{3a^2}\right) \\
								V &= 2V_1 + 2V_2 
										= 2\pi\left(\frac{3a^2b^2r - 2a^2r^3 - b^2r^3 + 2a^3b^2 - 3a^2b^2r + b^2r^3}{3a^2}\right) \\
									&= 2\pi\left(\frac{2a^3b^2 - 2a^2r^3}{3a^2}\right) 
										= 4\pi\left(\frac{ab^2 - r^3}{3}\right)
							\end{align*}
						\item
 							\begin{align*}
								V_1 &= \pi\int_0^r\left[\left(\sqrt{r^2 - x^2} - b\right)^2 - \left(\frac{b\sqrt{a^2 - x^2}}{a} - b\right)^2\right]\d x \\
									&= \pi\int_0^r\left[(r^2 - x^2) - 2b\sqrt{r^2 - x^2} + b^2 - \left(\frac{b^2(a^2 - x^2)}{a^2} -\frac{2b^2\sqrt{a^2 - x^2}}{a} + b^2\right)\right]\d x \\
									&= \pi\int_0^r\left[r^2 - x^2 - 2b\sqrt{r^2 - x^2} + b^2 - b^2 +  \frac{b^2x^2}{a^2} + \frac{2b^2\sqrt{a^2 - x^2}}{a} - b^2\right]\d x \\
									&= \pi\int_0^r\left[r^2 - x^2 - 2b\sqrt{r^2 - x^2} - b^2 + \frac{b^2x^2}{a^2} + \frac{2b^2\sqrt{a^2 - x^2}}{a}\right]\d x \\
									&= \pi\left(\left[(r^2 - b^2)x + \left(\frac{b^2}{a^2} - 1 \right)\frac{x^3}{3}\right]_0^r + 2b\int_0^r\left[\sqrt{r^2 - x^2} + \frac{\sqrt{a^2 - x^2}}{a}\right]\d x\right) \\
								I &= \int\left[\sqrt{\alpha^2 - x^2}\right]\d x 
										\implies x = \alpha\sin\theta 
										\implies \d x = \alpha\cos\theta\d\theta \\
									&= \int\left[\cos\theta\sqrt{\alpha^2 - \alpha^2\sin^2\theta}\right]\d\theta
										= \int\left[\alpha^2\cos^2\theta\right]\d\theta
										= \alpha^2\int\left[\frac{\cos(2\theta) + 1}{2}\right]\d\theta \\
									&= \alpha\left(\frac{\sin(2\theta)}{4} + \frac{\theta}{2}\right) + C
										= \alpha\left(\frac{2\sin\theta\cos\theta}{4} + \frac{\theta}{2}\right) + C \\
									&= \alpha^2\left(\frac{\left(\frac{x}{\alpha}\right)\left(\frac{\sqrt{\alpha^2 - x^2}}{\alpha}\right)}{2} + \frac{\arcsin(x/\alpha)}{2}\right) + C
										= \frac{x\sqrt{\alpha^2 - x^2} + \alpha^2\arcsin(x/\alpha)}{2} + C \\
								V_1 &= \begin{aligned}[t] &\pi\left[(r^2 - b^2)x + \left(\frac{b^2}{a^2} - 1 \right)\frac{x^3}{3}\right. \\ &\left.+ 2b\left(\frac{x\sqrt{r^2 - x^2} + r^2\arcsin(x/r)}{2} + \frac{x\sqrt{a^2 - x^2} + a^2\arcsin(x/a)}{2a}\right)\right]_0^r \end{aligned} \\
									&= \begin{aligned}[t]&\pi\left[x\left(r^2 - b^2 - \frac{x^2}{3}\left(\frac{b^2}{a^2} - 1\right)\right)\right. \\ &\left.+ \frac{b}{a}\left(x\left(\sqrt{r^2 - x^2} + \sqrt{a^2 - x^2}\right) + r^2\arcsin(x/r) + a^2\arcsin(x/a)\right)\right]_0^r\end{aligned} \\
									&= \begin{aligned}[t]&\pi\left[r\left(r^2 - b^2 - \frac{r^2}{3}\left(\frac{b^2}{a^2} - 1\right) \right)\right. \\ &\left.+ \frac{b}{a}\left(r\left(0 + \sqrt{a^2 - r^2}\right) + \frac{\pi r^2}{2} + a^2\arcsin\left(\frac{r}{a}\right)\right) - (0)\right]\end{aligned}\\
									&= \pi\left[\right]
							\end{align*}
					\end{enumerate}
			\end{enumerate}
	\chapter*{Indeterminate Exponents (Type 3)\markboth{Indeterminate Exponents}{}}
		\section*{Sources}
			\subsection*{Calculus: Early Transcendentals 9$^{\textbf{th}}$ Edition}
				\begin{enumerate}
					\item
						4.4 Exercise 61
					\item
						4.4 Exercise 57
					\item
						4.4 Exercise 60
					\item
						4.4 Exercise 65
					\item
						4.4 Exercise 66
				\end{enumerate}
			\newpage
		\section*{Problems}
			Evaluate the following limits.
			\begin{enumerate}
				\item
					\[\lim_{x\to 1^+}\left[x^{1/(1 - x)}]\right]\]
				\item
					\[\lim_{x\to 0^+}\left[x^{\sqrt{x}}\right]\]
				\item
					\[\lim_{x\to\infty}\left(1 + \frac{a}{x}\right)^{bx}\]
				\item
					\[\lim_{x\to 0^+}(4x + 1)^{\cot x}\]
				\item
					\[\lim_{x\to 0^+}(1 - \cos x)^{\sin x}\]
			\end{enumerate}
			\newpage
		\section*{Solutions}
			\begin{enumerate}
				\item
					\begin{align*}
						L &= \lim_{x\to 1^+}\left[x^{1/(1-x)}\right]
								&&\implies 1^{\infty} \\
						\ln L &= \lim_{x\to 1^+}\left[\frac{\ln x}{1 - x}\right]
								&&\implies \frac{0}{0} \\
							&= \lim_{x\to 1^+}\left[-\frac{1/x}{1}\right] 
								= -\frac{1/1}{1} = -1 \\
						L &= \frac{1}{e}
					\end{align*}
				\item
					\begin{align*}
						L &= \lim_{x\to 0^+}\left[x^{\sqrt{x}}\right] 
							&&\implies 0^0 \\
						\ln L &= \lim_{x\to 0^+}\left[\sqrt{x}\ln x\right] 
							&&\implies 0 \times (-\infty) \\
						&= \lim_{x\to 0^+}\left[\frac{\ln x}{x^{-1/2}}\right] 
							&&\implies -\frac{\infty}{\infty} \\
						&= \lim_{x\to 0^+}\left[-\frac{1/x}{0.5x^{-3/2}}\right] 
							= \lim_{x\to 0^+}\left[-2\sqrt{x}\right] = 0 \\
						L &= e^0 = 1
					\end{align*}
				\item
					\begin{align*}
						L &= \lim_{x\to\infty}\left(1 + \frac{a}{x}\right)^{bx}
								&&\implies 1^{\infty} \\
						\ln L &= \lim_{x\to\infty}\left[bx\ln\left(1 + \frac{a}{x}\right)\right]
								&&\implies \infty \times 0 \\
							&= \lim_{x\to\infty}\left[\frac{b\ln\left(1 + \frac{a}{x}\right)}{x^{-1}}\right]
								&&\implies \frac{0}{0} \\
							&= \lim_{x\to\infty}\left[\frac{\frac{-bax^{-2}}{1 + \frac{a}{x}}}{-x^{-2}}\right] 
								= \lim_{x\to\infty}\left[\frac{ab}{1 + \frac{a}{x}}\right] 
								= \frac{ab}{1 + 0} = ab \\
						L &= e^{ab}
					\end{align*}
				\item
					\begin{align*}
						L &= \lim_{x\to 0^+}(4x + 1)^{\cot x}
								&&\implies 1^{\infty} \\
						\ln L &= \lim_{x\to 0^+}[(\cot x)\ln(4x + 1)]
								&&\implies \infty \times 0 \\
							&= \lim_{x\to 0^+}\left[\frac{\ln(4x + 1)}{\tan x}\right]
								&&\implies \frac{0}{0} \\
							&= \lim_{x\to 0^+}\left[\frac{4/(x + 1)}{\sec^2 x}\right] 
								= \frac{4/1}{1} 
								= 4 \\
						L &= e^4
					\end{align*}
				\item
					\begin{align*}
						L &= \lim_{x\to 0^+}(1 - \cos x)^{\sin x}
								&&\implies 0^0 \\
						\ln L &= \lim_{x\to 0^+}\left[(\sin x)\ln(1 - \cos x)\right]
								&&\implies 0 \times (-\infty) \\
							&= \lim_{x\to 0^+}\left[\frac{\ln(1 - \cos x)}{\csc x}\right]
								&&\implies -\frac{\infty}{\infty} \\
							&= \lim_{x\to 0^+}\left[-\frac{\sin x /(1 - \cos x)}{\csc x \cot x}\right]
								= \lim_{x\to 0^+}\left[-\frac{\sin^2x\tan x}{1 - \cos x}\right]
								&&\implies -\frac{0}{0} \\
							&= \lim_{x\to 0^+}\left[\frac{2\sin x \cos x \tan x + \sin^2 x \sec^2 x}{\sin x}\right]
								= \lim_{x\to 0^+}[2\cos x \tan x + \sin x \sec x] \\
							&= 2(1)(0) + (0)(1) = 0 \\
						L &= 1
					\end{align*}
			\end{enumerate}
\end{document}