\documentclass[12pt]{article}

% Packages
	% Basics
		\usepackage{amsmath}
    	\usepackage{bm}
		\usepackage[shortlabels]{enumitem}
		\usepackage[margin = 1 in]{geometry}
	% Notation
		\usepackage{amssymb}
		\usepackage{esint}
		\usepackage{mathrsfs}
		\usepackage{physics}
    	\usepackage{siunitx}
% Macros
	\newcommand{\Ell}{\mathscr{L}}
	\newcommand{\en}{\text{e}}
  	\newcommand{\subt}[2]{#1_{\text{#2}}}
  	\newcommand{\Z}{\mathbb{Z}}
% Configuration
	\title{Discussion 12: Transform \(y\), \(y'\), \(y''\), \(y'''\), \(y''''\)}
	\author{Arnav Patri}
	
\begin{document}
	\maketitle
	\begin{enumerate}
		\item
			By definition,
				\[
					\Ell\{y\} = \int_0^\infty \en^{-st}y\dd{t}
						= Y(s)
				\]
		\item
			\begin{align*}
				\Ell\{y'\} &= \int_0^\infty \en^{-st}y'\dd{t} \tag{definition of \(\Ell\)} \\
					&= \left[\en^{-st}y\right]_0^\infty + \int_0^\infty s\en^{-st}y\dd{t} \tag{integration by parts} \\
					&= -y_0 + s\Ell\{y\} \tag{definition of \(\Ell\)} \\
					&= sY(s) - y_0
			\end{align*}
		\item
			\begin{align*}
				\Ell\{y''\} &= \int_0^\infty \en^{-st}y'' \dd{t} \tag{definition of \(\Ell\)} \\
					&= \left[\en^{-st}y'\right]_0^\infty + \int_0^\infty s\en^{-st}y' \dd{t} \tag{integration by parts} \\
					&= -y'_0 + s\Ell\{y'\} \tag{definition of \(\Ell\)} \\
					&= -y'_0 + s^2Y(s) - sy_0 \tag{substituting \(\Ell\{y'\}\)} \\
					&= s^2Y(s) - sy_0 - y'_0
			\end{align*}
		\item
			\begin{align*}
				\Ell\{y'''\} &= \int_0^\infty \en^{-st}y'' \dd{t} \tag{definition of \(\Ell\)} \\
					&= \left[\en^{-st}y''\right]_0^\infty + \int_0^\infty s\en^{-st}y'' \dd{t} \tag{integration by parts} \\
					&= -y''_0 + s\Ell\{y''\} \tag{definition of \(\Ell\)} \\
					&= -y''_0 + s^3Y(s) - s^2y_0 - sy'_0 \tag{substituting \(\Ell\{y''\}\)} \\
					&= s^3Y(s) - s^2y_0 - sy'_0 - y''_0
			\end{align*}
		\item
			\begin{align*}
				\Ell\{y''''\} &= \int_0^\infty \en^{-st}y''' \dd{t} \tag{definition of \(\Ell\)} \\
					&= \left[\en^{-st}y'''\right]_0^\infty + \int_0^\infty s\en^{-st}y''' \dd{t} \tag{integration by parts} \\
					&= -y'''_0 + s\Ell\{y'''\} \tag{definition of \(\Ell\)} \\
					&= -y'''_0 + s^4Y(s) - s^3y_0 - s^2y'_0 - sy''0\tag{substituting \(\Ell\{y'''\}\)} \\
					&= s^4Y(s) - s^3y_0 - s^2y'_0 - sy''_0 - y'''_0
			\end{align*}
	\end{enumerate}
\end{document}