\documentclass[12pt]{article}

% Packages
	% Basics
		\usepackage{amsmath}
    	\usepackage{bm}
		\usepackage[shortlabels]{enumitem}
		\usepackage[margin = 1 in]{geometry}
	% Notation
		\usepackage{amssymb}
		\usepackage{esint}
		\usepackage{mathrsfs}
		\usepackage{physics}
    	\usepackage{siunitx}
% Macros
	\newcommand{\Ell}{\mathscr{L}}
	\newcommand{\en}{\text{e}}
  	\newcommand{\subt}[2]{#1_{\text{#2}}}
  	\newcommand{\Z}{\mathbb{Z}}
% Configuration
	\title{Transform from a function of \(t\) to a function of \(s\)}
	\author{Arnav Patri}

\begin{document}
	\maketitle
	\thispagestyle{empty}
	\begin{enumerate}[1)]
		\item
			\begin{align*}
				\Ell\{\en^{3t}\} &= \int_0^\infty \en^{-st}\en^{3t}\dd{t}
						= \int_0^\infty \en^{-t(s - 3)}\dd{t} 
						= \left[-\frac{\en^{-t(s - 3)}}{(s - 3)}\right]_0^\infty \\
					&= 0 + \frac{1}{s - 3}
						= \frac{1}{s - 3}
			\end{align*}
			Using theorem 7.1.1,
				\[\Ell\{e^{3t}\} = \frac{1}{s - 3}\]
		\item
			\[\Ell\{f(t)\} = \int_0^\infty \en^{-st}f(t)\dd{t} = F(s)\]
		\item
			Using theorem 7.1.1,
			\[
				\Ell\{\sin(3t)\} = \frac{3}{s^2 + 3^2}
					= \frac{3}{s^2 + 9}
			\]
		\item
			Using theorem 7.1.1,
			\[
				\Ell\{\cos^2(2t)\} = \Ell\left\{\frac{1 + \cos(4x)}{2}\right\}
					= \frac{1}{2}\frac{1}{s} + \frac{1}{2}\frac{s}{s^2 + 4^2}
					= \frac{1}{2s} + \frac{s}{2s^2 + 32}
					= \frac{s^2 + 8}{s^3 + 16s}
			\]
	\end{enumerate}
\end{document}