\documentclass{article}[A4, 12pt]

\usepackage{amsmath}
\usepackage{amssymb}
\usepackage[margin = 0.75 in]{geometry}

% Configuration
\title{Assignment 2}
\author{Arnav Patri}

% Notation
\renewcommand{\Vec}[1]{\overrightarrow{#1}}
\newcommand{\vi}{\text{\^\i}}
\newcommand{\vj}{\text{\^\j}}
\newcommand{\vk}{\text{\^k}}

\begin{document}
	\maketitle
	\begin{enumerate}
		\item
			Find the angle between the vectors $\vec{a} = \vi - 2\vj + \vk$ and $\vec{b} = 2\vi + \vj - \vk$.
			\subitem
				\textbf{Solution:}
					\begin{align*}
						|\vec{a}||\vec{b}|\cos\theta &= \vec{a} \cdot \vec{b} \\
						\sqrt{1^2 + (-2)^2 + (1)^2}\sqrt{2^2 + 1^2 + (-1)^2}\cos\theta	&= (1)(2) + (-2)(1) + (1)(-1) \\
						\sqrt{6}\sqrt{6}\cos\theta &= -1 \\
						\theta &= \arccos\left(-\frac{1}{6}\right) \approx 100^{\circ}
					\end{align*}
		\item
			Find the cross product of the vectors $\vec{a} = \langle 2, -1, 4 \rangle$ and $\vec{b} = \langle 3, 0, -2 \rangle$.
			\subitem
				\textbf{Solution:}
					\begin{align*}
						\vec{a} \times \vec{b} 
							&= \begin{vmatrix}
							 \vi & \vj & \vk \\
							 2 & -1 & 4 \\
							 3 & 0 & -2
							\end{vmatrix} 
								= \langle (-1)(-2) - (4)(0), -1((2)(-2) - (4)(3)), (2)(0) - (-1)(3) \rangle
								= \langle 2, 16, 3 \rangle
					\end{align*}
		\item
			Find the equation of the plane $Ax + By + Cz = D$ through the points $P(1, -1, 2)$, $Q(-1, 0, 1)$, and $R(1, -1, 1)$.
			\subitem
				\textbf{Solution}
					\begin{align*}
						\Vec{PQ} &= \langle -1 -1, 0 - (-1), 1 - 2 \rangle 
								= \langle -2, 1, -1 \rangle \\
						\Vec{PR} &= \langle 1 - 1, -1 - (-1), 1 - 2 \rangle
								= \langle 0, 0, -1 \rangle \\
						\vec{n} &= \Vec{PQ} \times \Vec{PR}
								= \begin{vmatrix}
	 								\vi & \vj & \vk \\
	 								-2 & 1 & -1 \\
	 								0 & 0 & -1
	 							\end{vmatrix}
	 							= \langle (1)(-1) - (-1)(0), -1((-2)(-1) - (-1)(0)), (-2)(0) - (-1)(0) \rangle 
	 							= \langle -1, -2, 0 \rangle \\
	 					D &= n_xx + n_yy + n_zz 
	 							= -1(1) + (-2)(-1) + 0(2)
	 							= -1 + 2 + 0
	 							= 1 \\
	 					1 &= -x - 2y 
					\end{align*}
	\end{enumerate}
\end{document}